Phi_System/IDE_CP_Core.thy
@@ -1613,7 +1613,7 @@ lemma \<phi>apply_proc_fully[\<phi>reason %\<phi>app_proc_on_proc_or_VS for
 ]:
   \<open> \<phi>IntroFrameVar' R S'' S' T T' E'' E'
 \<Longrightarrow> S \<t>\<r>\<a>\<n>\<s>\<f>\<o>\<r>\<m>\<s> S'' \<w>\<i>\<t>\<h> P @action NToA
-\<Longrightarrow> Simplify (assertion_simps undefined) E''' E''
+\<Longrightarrow> Simplify (assertion_simps ABNORMAL) E''' E''
 \<Longrightarrow> (\<And>v. Remove_Values (E''' v) (E v))
 \<Longrightarrow> \<o>\<b>\<l>\<i>\<g>\<a>\<t>\<i>\<o>\<n> True
 \<Longrightarrow> PROP \<phi>Application (Trueprop (\<p>\<r>\<o>\<c> f \<lbrace> S' \<longmapsto> T' \<rbrace> \<t>\<h>\<r>\<o>\<w>\<s> E' ))
